Prove lemma 9.5 under some assumptions

PolymorphicTypeSystem.v
@@ -241,6 +241,31 @@ Proof.
         apply (Sub_List _ _ _ Ht0').
 Qed.
 
+Lemma subst_scheme_close :
+    forall (S : TySubst) (s : TyScheme),
+    exists s' : TyScheme, subst_scheme S s s'.
+Proof.
+Admitted.
+
+Lemma subst_env_close :
+    forall (S : TySubst) (C : TEnv),
+    exists C' : TEnv, subst_env S C C'.
+Proof.
+    intros S C.
+    induction C as [ | C0 HC0 x s ].
+
+        (* Case : C = TEEmpty *)
+        exists TEEmpty.
+        apply Sub_Empty.
+
+        (* Case : C = TEBind C0 x s *)
+        destruct HC0 as [C0' HC0'].
+        remember (subst_scheme_close S s) as Hs'; clear HeqHs'.
+        destruct Hs' as [s' Hs'].
+        exists (TEBind C0' x s').
+        apply (Sub_Bind _ _ _ _ _ _ HC0' Hs').
+Qed.
+
 (* Lemma 9.3 *)
 Lemma Typable_subst_compat :
     forall (C C' : TEnv) (e : Exp) (t t' : Types) (S : TySubst),
@@ -346,6 +371,93 @@ Proof.
 
         (* Case : e = EMatch x y e1 e2 e3 *)
         admit.
+Qed.
+
+(* Def 9.4 *)
+Inductive ValueCompat : Value -> Types -> Prop :=
+    | VC_Int    : forall i : Z, ValueCompat (VInt i) TInt
+    | VC_Bool   : forall b : bool, ValueCompat (VBool b) TBool
+    | VC_Fun    : forall (E : Env) (C : TEnv) (e : Exp)
+                         (x : Var) (t1 t2 : Types),
+                  EnvCompat E C -> Typable (TEBind C x (TSType t1)) e t2 ->
+                  ValueCompat (VFun E x e) (TFun t1 t2)
+    | VC_RecFun : forall (E : Env) (C : TEnv) (e : Exp)
+                         (x y : Var) (t1 t2 : Types),
+                  EnvCompat E C ->
+                  Typable (TEBind (TEBind C x (TSType (TFun t1 t2)))
+                                            y (TSType t1))
+                          e t2 ->
+                  ValueCompat (VRecFun E x y e) (TFun t1 t2)
+    | VC_Nil    : forall t' : Types, ValueCompat VNil (TList t')
+    | VC_Cons   : forall (t' : Types) (v1 v2 : Value),
+                  ValueCompat v1 t' -> ValueCompat v2 (TList t') ->
+                  ValueCompat (VCons v1 v2) (TList t')
+    with EnvCompat : Env -> TEnv -> Prop :=
+    | EC_Empty : EnvCompat EEmpty TEEmpty
+    | EC_Bind  : forall (E' : Env) (C' : TEnv)
+                        (x : Var) (v : Value) (s : TyScheme) (t : Types),
+                 EnvCompat E' C' -> ValueCompat v t -> is_type s t ->
+                 EnvCompat (EBind E' x v) (TEBind C' x s).
+
+Lemma EnvCompat_subst_compat :
+    forall (S : TySubst) (E : Env) (C C' : TEnv),
+    EnvCompat E C -> subst_env S C C' -> EnvCompat E C'.
+Proof.
+Admitted.
+
+(* Lemma 9.5 *)
+Lemma ValueCompat_subst_compat :
+    forall (S : TySubst) (v : Value) (t t' : Types),
+    ValueCompat v t -> subst_type S t t' -> ValueCompat v t'.
+Proof.
+    intros S v.
+    induction v as [ i | b | E x e0 | E x y e0 | | v1 Hv1 v2 Hv2 ].
+
+        (* Case : v = VInt i *)
+        intros t t' Hvc Hst.
+        inversion Hvc; subst.
+        inversion Hst; subst.
+        apply VC_Int.
+
+        (* Case : v = VBool b *)
+        intros t t' Hvc Hst.
+        inversion Hvc; subst.
+        inversion Hst; subst.
+        apply VC_Bool.
+
+        (* Case : v = VFun E x e0 *)
+        intros t t' Hvc Hst.
+        inversion Hvc; subst.
+        inversion Hst; subst.
+        remember (subst_env_close S C) as HC'; clear HeqHC'.
+        destruct HC' as [C' HC'].
+        apply (VC_Fun _ _ _ _ _ _ (EnvCompat_subst_compat _ _ _ _ H3 HC')).
+        refine (Typable_subst_compat _ _ _ _ _ _ H4 _ H6).
+        apply (Sub_Bind _ _ _ _ _ _ HC' (Sub_Type _ _ _ H2)).
+
+        (* Case : v = VRecFun E x y e0 *)
+        intros t t' Hvc Hst.
+        inversion Hvc; subst.
+        inversion Hst; subst.
+        remember (subst_env_close S C) as HC'; clear HeqHC'.
+        destruct HC' as [C' HC'].
+        apply (VC_RecFun _ _ _ _ _ _ _ (EnvCompat_subst_compat _ _ _ _ H4 HC')).
+        refine (Typable_subst_compat _ _ _ _ _ _ H5 _ H6).
+        refine (Sub_Bind _ _ _ _ _ _ _ (Sub_Type _ _ _ H2)).
+        apply (Sub_Bind _ _ _ _ _ _ HC'
+                        (Sub_Type _ _ _ (Sub_Fun _ _ _ _ _ H2 H6))).
+
+        (* Case : v = VNil *)
+        intros t t' Hvc Hst.
+        inversion Hvc; subst.
+        inversion Hst; subst.
+        apply VC_Nil.
+
+        (* Case : v = VCons v1 v2 *)
+        intros t t' Hvc Hst.
+        inversion Hvc; subst.
+        inversion Hst; subst.
+        apply (VC_Cons _ _ _ (Hv1 _ _ H1 H2) (Hv2 _ _ H3 (Sub_List _ _ _ H2))).
 Qed.
 
 End PolymorphicTypeSystem.
